File clean up and added determinism and subset proofs
Two new files were added. These are "UpdateSemHelper.thy" and
"ValueSemHelper.thy". These two files contain helper lemmas and
definitions that are not specific to repeat.

Proofs showing that the update and value semantics are deterministic
if the abstract functions are deterministic were added.

Proofs showing that evaluation and preservation of abstract functions
in the update and value semantics are occurs for the same expressions
and arguments for an abstract function environment (xi) if it occurs
for a smaller abstract function environment were added.

Similarly, proofs for corres and correspondence of abstract functions
(for certain cases) were also added.

cogent/examples/repeat/RepeatAssm.thy
@@ -1,5 +1,8 @@
 theory RepeatAssm
-  imports "build/Generated_AllRefine"
+  imports
+    UpdateSemHelper
+    ValueSemHelper
+    "build/Generated_AllRefine"
 begin
 
 section "C helpers"
@@ -37,94 +40,6 @@ lemma proc_ctx_wellformed_\<Xi>:
             log2stop_type_def log2step_type_def mylog2_type_def
   by (clarsimp simp: assoc_lookup.simps)
 
-
-section "update semantics helpers"
-
-inductive_cases u_sem_appE: "\<xi>',\<gamma> \<turnstile> (\<sigma>,App x y)\<Down>! (\<sigma>',v)"
-inductive_cases u_sem_funE: "\<xi>',\<gamma> \<turnstile> (\<sigma>,Fun x y)\<Down>! (\<sigma>',v)"
-inductive_cases u_sem_afunE: "\<xi>',\<gamma> \<turnstile> (\<sigma>,AFun x y)\<Down>! (\<sigma>',v)"
-inductive_cases u_sem_primE: "\<xi>',\<gamma> \<turnstile> (\<sigma>,Prim x y)\<Down>! (\<sigma>',v)"
-inductive_cases u_sem_consE: "\<xi>',\<gamma> \<turnstile>* (\<sigma>,xs)\<Down>! (\<sigma>',v)"
-
-context update_sem begin
-
-lemma frame_empty:
-  "frame \<sigma> {} \<sigma>' {} \<Longrightarrow> \<sigma> = \<sigma>'"
-  apply (clarsimp simp: frame_def fun_eq_iff)
-  done
-
-lemma discardable_or_shareable_not_writable:
-assumes "D \<in> k \<or> S \<in> k"
-shows "\<lbrakk> \<Xi>', \<sigma> \<turnstile>  v  :u  \<tau>  \<langle> r , w \<rangle>; K' \<turnstile>  \<tau>  :\<kappa>  k \<rbrakk> \<Longrightarrow> w = {}"
-and   "\<lbrakk> \<Xi>', \<sigma> \<turnstile>* fs :ur \<tau>s \<langle> r , w \<rangle>; K' \<turnstile>* \<tau>s :\<kappa>r k \<rbrakk> \<Longrightarrow> w = {}"
-  using assms
-  by (induct rule: uval_typing_uval_typing_record.inducts)
-    (force simp add: kinding_simps kinding_record_simps kinding_variant_set
-      dest: abs_typing_readonly[where s = Unboxed,simplified])+
-
-lemma discardable_or_shareable_not_writable':
-shows "\<lbrakk> k = kinding_fn K' \<tau>; D \<in> k \<or> S \<in> k; \<Xi>', \<sigma> \<turnstile>  v  :u  \<tau>  \<langle> r , w \<rangle>; K' \<turnstile>  \<tau>  :\<kappa> k \<rbrakk> \<Longrightarrow> w = {}"
-and   "\<lbrakk> k = (\<Inter>(_,t,b)\<in>set \<tau>s. (case b of Taken \<Rightarrow> UNIV | Present \<Rightarrow> kinding_fn K' t));
-         D \<in> k \<or> S \<in> k; \<Xi>', \<sigma> \<turnstile>* fs :ur \<tau>s \<langle> r , w \<rangle>; K' \<turnstile>* \<tau>s :\<kappa>r k \<rbrakk> \<Longrightarrow> w = {}"
-  by (meson discardable_or_shareable_not_writable)+
-
-lemma bang_not_writable:
-shows "\<lbrakk> \<Xi>', \<sigma> \<turnstile>  v  :u  bang \<tau>  \<langle> r , w \<rangle> \<rbrakk> \<Longrightarrow> w = {}"
-and   "\<lbrakk> \<Xi>', \<sigma> \<turnstile>* fs :ur map (\<lambda>(n, t, b). (n, bang t, b)) \<tau>s \<langle> r , w \<rangle>  \<rbrakk> \<Longrightarrow> w = {}"
-  apply (frule discardable_or_shareable_not_writable'(1)[where K' = "[]", simplified, rotated -2]; simp?)
-    apply (rule kindingI[OF uval_typing_to_wellformed(1)]; simp?)
-   apply (cut_tac K = "[]" and t = \<tau> in bang_kinding_fn; clarsimp)
-  apply (frule discardable_or_shareable_not_writable'(2)[where K' = "[]", simplified, rotated -2]; simp?)
-  apply (frule uval_typing_to_wellformed(2))
-   apply (clarsimp simp: kinding_record_def)
-  apply (rename_tac a aa b)
-   apply (erule_tac x = "(a, aa, b)" in ballE; clarsimp)
-  apply (clarsimp split: record_state.splits)
-  apply (rename_tac a aa ab ac)
-  apply (cut_tac K = "[]" and t = ac in bang_kinding_fn; clarsimp)
-  done
-
-definition \<xi>ule :: "('f, 'a, 'l) uabsfuns \<Rightarrow> ('f, 'a, 'l) uabsfuns \<Rightarrow> bool"
-  where
-"\<xi>ule f g = ({(n, a, b) | n a b. f n a b} \<subseteq> {(n, a, b) | n a b. g n a b})"
-
-lemma \<xi>vle_matches:
-  "\<lbrakk>\<xi>b matches-u \<Xi>'; \<xi>ule \<xi>a \<xi>b\<rbrakk> \<Longrightarrow> \<xi>a matches-u \<Xi>'"
-  unfolding proc_env_matches_ptrs_def \<xi>ule_def
-  apply clarsimp
-  apply (erule_tac x = f in allE; clarsimp)
-  apply (erule_tac x = \<sigma> in allE)
-  apply (erule_tac x = \<sigma>' in allE)
-  apply (erule_tac x = \<tau>s in allE; clarsimp)
-  apply (erule_tac x = v in allE)
-  apply (erule_tac x = v' in allE)
-  apply (erule_tac x = r in allE)
-  apply (erule_tac x = w in allE; clarsimp)
-  apply (drule_tac c = "(f, (\<sigma>, v), (\<sigma>', v'))" in  subsetD; simp)
-  done
-
-end (* of context *)
-
-section "value semantics helpers"
-
-context value_sem begin
-
-definition \<xi>vle :: "('f, 'a) vabsfuns \<Rightarrow> ('f, 'a) vabsfuns \<Rightarrow> bool"
-  where
-"\<xi>vle f g = ({(n, a, b) | n a b. f n a b} \<subseteq> {(n, a, b) | n a b. g n a b})"
-
-lemma \<xi>vle_matches:
-  "\<lbrakk>\<xi>b matches \<Xi>'; \<xi>vle \<xi>a \<xi>b\<rbrakk> \<Longrightarrow> \<xi>a matches \<Xi>'"
-  unfolding proc_env_matches_def \<xi>vle_def
-  apply clarsimp
-  apply (erule_tac x = f in allE; clarsimp)
-  apply (erule_tac x = \<tau>s in allE; clarsimp)
-  apply (erule_tac x = v in allE; clarsimp)
-  apply (erule_tac x = v' in allE; clarsimp)
-  apply (drule_tac c = "(f, v, v')" in  subsetD; simp)
-  done
-
-end (* of context *)
 
 section "correspondence helpers"
 
@@ -167,8 +82,8 @@ and   "\<lbrakk> \<Xi>', \<sigma> \<turnstile>* fs \<sim> fs' :r map (\<lambda>(
   done
 
 lemma \<xi>ule_matchesuv:
-  "\<lbrakk>\<xi>ub \<sim> \<xi>v matches-u-v \<Xi>'; upd.\<xi>ule \<xi>ua \<xi>ub\<rbrakk> \<Longrightarrow> \<xi>ua \<sim> \<xi>v matches-u-v \<Xi>'"
-  unfolding proc_env_u_v_matches_def upd.\<xi>ule_def
+  "\<lbrakk>\<xi>ub \<sim> \<xi>v matches-u-v \<Xi>'; \<xi>ule \<xi>ua \<xi>ub\<rbrakk> \<Longrightarrow> \<xi>ua \<sim> \<xi>v matches-u-v \<Xi>'"
+  unfolding proc_env_u_v_matches_def \<xi>ule_def
   apply clarsimp
   apply (erule_tac x = f in allE; clarsimp)
   apply (erule_tac x = \<sigma> in allE)
@@ -183,8 +98,65 @@ lemma \<xi>ule_matchesuv:
   apply (drule_tac c = "(f, (\<sigma>, aa), (\<sigma>', v))" in  subsetD; simp)
   done
 
+definition proc_env_u_v_matches_alt :: "(('f, 'au, 'l) uabsfuns)
+
+                                  \<Rightarrow> (('f, 'av)    vabsfuns)
+                                  \<Rightarrow> ('f \<Rightarrow> poly_type)
+                                  \<Rightarrow> bool"
+           ("_ \<sim> _ altmatches-u-v _" [30,20] 60) where
+  "\<xi>u \<sim> \<xi>v altmatches-u-v \<Xi>'
+          \<equiv> (\<forall> f. let (K, \<tau>i, \<tau>o) = \<Xi>' f
+                  in (\<forall> \<sigma> \<sigma>' \<tau>s a a' v r w.
+                         list_all2 (kinding []) \<tau>s K
+                      \<longrightarrow> (\<Xi>' , \<sigma> \<turnstile> a \<sim> a' : instantiate \<tau>s \<tau>i \<langle>r, w\<rangle>)
+                      \<longrightarrow> \<xi>u f (\<sigma>, a) (\<sigma>', v)
+                      \<longrightarrow> (\<exists>v'. \<xi>v f a' v' \<and> 
+                            (\<exists>r' w'. (\<Xi>' , \<sigma>' \<turnstile> v \<sim> v' : instantiate \<tau>s \<tau>o \<langle>r', w'\<rangle>)
+                                    \<and> r' \<subseteq> r \<and> upd.frame \<sigma> w \<sigma>' w'))))"
+
+lemma 
+  "\<xi>u \<sim> \<xi>v matches-u-v \<Xi>' \<Longrightarrow> \<xi>u \<sim> \<xi>v altmatches-u-v \<Xi>'"
+  unfolding proc_env_u_v_matches_def proc_env_u_v_matches_alt_def
+  apply (clarsimp split: prod.splits)
+  apply (elim allE, erule impE, assumption)
+  apply (erule_tac x = \<sigma> in allE)
+  apply (erule_tac x = \<sigma>' in allE)
+  apply (elim allE, erule impE, assumption)
+  apply (erule allE, erule_tac x = a' in allE, elim allE, erule impE, assumption)
+  apply (subst (asm) all_comm)
+  apply (erule_tac x = r in allE)
+  apply (subst (asm) all_comm)
+  apply (erule_tac x = w in allE)
+  apply clarsimp
+  apply (elim allE impE, assumption)
+  apply clarsimp
+  apply (intro exI conjI; assumption)
+  done
+
 end (* of context *)
 
 section "monomorphisation helpers"
+
+context value_sem begin
+thm rename_mono_prog_def
+end
+
+section "corres helpers"
+
+context update_sem_init begin
+
+lemma corres_\<xi>ule:
+  "\<lbrakk>corres srel c m \<xi>a \<gamma> \<Xi>' \<Gamma> \<sigma> s; \<xi>ule \<xi>a \<xi>b\<rbrakk> \<Longrightarrow> corres srel c m \<xi>b \<gamma> \<Xi>' \<Gamma> \<sigma> s"
+  unfolding corres_def
+  apply clarsimp
+  apply (erule impE, rule \<xi>ule_matches, assumption, assumption)
+  apply (erule impE, intro exI, assumption)
+  apply clarsimp
+  apply (elim allE, erule impE, assumption)
+  apply clarsimp
+  apply (drule u_sem_u_sem_all_\<xi>ule; simp?)
+  apply (intro exI conjI; assumption)
+  done
+end (* of context *)
 
 end
