cogent/examples/repeat/ValueSemHelper.thy
@@ -1,0 +1,219 @@
+theory ValueSemHelper
+  imports "Cogent.ValueSemantics"
+begin
+section "value semantics helpers"
+
+definition \<xi>vle :: "('f, 'a) vabsfuns \<Rightarrow> ('f, 'a) vabsfuns \<Rightarrow> bool"
+  where
+"\<xi>vle f g = ({(n, a, b) | n a b. f n a b} \<subseteq> {(n, a, b) | n a b. g n a b})"
+
+lemma v_sem_v_sem_all_\<xi>vle:
+  shows "\<lbrakk>\<xi>a, \<gamma> \<turnstile> e  \<Down> v; \<xi>vle \<xi>a \<xi>b\<rbrakk> \<Longrightarrow> \<xi>b, \<gamma> \<turnstile> e \<Down> v"
+  and "\<lbrakk>\<xi>a , \<gamma> \<turnstile>* es \<Down> vs; \<xi>vle \<xi>a \<xi>b\<rbrakk> \<Longrightarrow> \<xi>b , \<gamma> \<turnstile>* es \<Down> vs"
+proof (induct arbitrary: \<xi>b and \<xi>b rule: v_sem_v_sem_all.inducts)
+  case (v_sem_abs_app \<xi> \<gamma> x f ts y a r)
+  then show ?case
+    apply -
+    apply (drule_tac x = \<xi>b in meta_spec; simp?)+
+    apply (rule v_sem_v_sem_all.v_sem_abs_app; simp?)
+    unfolding \<xi>vle_def by blast
+next
+  case (v_sem_app \<xi> \<gamma> x e ts y a r)
+  then show ?case
+    apply -
+    apply (drule_tac x = \<xi>b in meta_spec; simp?)+
+    by (rule v_sem_v_sem_all.v_sem_app; simp?)
+qed (auto intro: v_sem_v_sem_all.intros)
+
+definition \<xi>v_determ :: "('f, 'a) vabsfuns \<Rightarrow> bool"
+  where
+"\<xi>v_determ \<xi>v = (\<forall>f a b c. \<xi>v f a b \<and>  \<xi>v f a c \<longrightarrow> b = c)"
+
+lemma
+  "\<not> \<xi>v_determ (\<lambda>f a b. (b = VPrim (LBool True)) \<or> (b = VPrim (LBool False)))"
+  unfolding \<xi>v_determ_def
+  apply clarsimp
+  apply (rule_tac x = "VPrim (LBool True)" in exI; clarsimp)
+  apply (rule_tac x = "VPrim (LBool False)" in exI; clarsimp)
+  done
+
+lemma
+  "\<xi>v_determ (\<lambda>f a b. b = VUnit)"
+  unfolding \<xi>v_determ_def
+  by clarsimp
+
+inductive_cases v_sem_letE: "\<xi> , \<gamma> \<turnstile> Let a b \<Down> b'"
+inductive_cases v_sem_letBangE: "\<xi> , \<gamma> \<turnstile> LetBang vs a b \<Down> b'"
+inductive_cases v_sem_litE: "\<xi> , \<gamma> \<turnstile> Lit l \<Down> v"
+inductive_cases v_sem_primE: "\<xi> , \<gamma> \<turnstile> Prim p as \<Down> r"
+inductive_cases v_sem_memberE: "\<xi> , \<gamma> \<turnstile> Member x f \<Down> r"
+inductive_cases v_sem_tupleE: "\<xi> , \<gamma> \<turnstile> Tuple a b \<Down> r"
+inductive_cases v_sem_ifE: " \<xi> , \<gamma> \<turnstile> If x t e \<Down> r"
+inductive_cases v_sem_conE: "\<xi> , \<gamma> \<turnstile> Con i t x \<Down> r"
+inductive_cases v_sem_esacE: "\<xi>, \<gamma> \<turnstile> Esac v  n \<Down> r"
+inductive_cases v_sem_caseE:  "\<xi> , \<gamma> \<turnstile> Case x c m n \<Down> r"
+inductive_cases v_sem_splitE: "\<xi> , \<gamma> \<turnstile> Split x e \<Down> e'"
+inductive_cases v_sem_takeE: "\<xi> , \<gamma> \<turnstile> Take x f e \<Down> e'"
+inductive_cases v_sem_putE: "\<xi> , \<gamma> \<turnstile> Put x f e \<Down> e'"
+inductive_cases v_sem_castE: "\<xi> , \<gamma> \<turnstile> Cast \<tau> e \<Down> e'"
+inductive_cases v_sem_structE: "\<xi> , \<gamma> \<turnstile> Struct ts xs \<Down> e'"
+inductive_cases v_sem_AppE: "\<xi> , \<gamma> \<turnstile> App f v \<Down> e'"
+inductive_cases v_sem_allE: "\<xi> , \<gamma> \<turnstile>* es \<Down> es'"
+inductive_cases v_sem_all_NilE: "\<xi> , \<gamma> \<turnstile>* [] \<Down> es'"
+inductive_cases v_sem_all_ConsE: "\<xi> , \<gamma> \<turnstile>* (e#es) \<Down> es'"
+inductive_cases v_sem_unitE: "\<xi> , \<gamma> \<turnstile> Unit \<Down> r"
+inductive_cases v_sem_promoteE: "\<xi>, \<gamma> \<turnstile> Promote \<tau> e \<Down> r"
+
+lemmas v_sem_elims =
+  v_sem_letE
+  v_sem_letBangE
+  v_sem_litE
+  v_sem_primE
+  v_sem_memberE
+  v_sem_tupleE
+  v_sem_ifE
+  v_sem_conE
+  v_sem_esacE
+  v_sem_caseE
+  v_sem_splitE
+  v_sem_takeE
+  v_sem_putE
+  v_sem_castE
+  v_sem_structE
+  v_sem_AppE
+  v_sem_allE
+  v_sem_all_NilE
+  v_sem_all_ConsE
+  v_sem_unitE
+  v_sem_promoteE
+
+lemma v_sem_v_sem_all_determ:
+  shows "\<lbrakk>\<xi>a, \<gamma> \<turnstile> e  \<Down> v; \<xi>a, \<gamma> \<turnstile> e \<Down> v'; \<xi>v_determ \<xi>a\<rbrakk> \<Longrightarrow> v = v'"
+  and "\<lbrakk>\<xi>a , \<gamma> \<turnstile>* es \<Down> vs; \<xi>a , \<gamma> \<turnstile>* es \<Down> vs'; \<xi>v_determ \<xi>a\<rbrakk> \<Longrightarrow> vs = vs'"
+proof (induct arbitrary: v' and vs' rule: v_sem_v_sem_all.inducts)
+  case (v_sem_abs_app \<xi> \<gamma> x f ts y a r)
+  then show ?case 
+    apply -
+    apply (erule v_sem_appE; simp?)    
+     apply (rename_tac f' ts' a')
+     apply (drule_tac x = "VAFunction f' ts'" in meta_spec; clarsimp)
+     apply (drule_tac x = a' in meta_spec; clarsimp)
+    unfolding \<xi>v_determ_def
+     apply (erule_tac x = f in allE)
+     apply (erule_tac x = a in allE)
+     apply (erule_tac x = r in allE)
+     apply (erule_tac x = v' in allE)
+     apply (erule impE; simp)
+     apply (rename_tac f' ts' a')
+     apply (drule_tac x = "VFunction f' ts'" in meta_spec; clarsimp)
+    done
+next
+  case (v_sem_app \<xi> \<gamma> x e ts y a r)
+  then show ?case
+    apply -
+    apply (erule v_sem_appE)
+     apply (rename_tac f' ts' a')
+     apply (drule_tac x = "VAFunction f' ts'" in meta_spec)
+     apply (elim meta_impE; assumption?)
+     apply blast
+    apply (rename_tac f' ts' a')
+    apply (drule_tac x = "VFunction f' ts'" in meta_spec)
+    apply (elim meta_impE; assumption?)
+    apply (drule_tac x = a' in meta_spec; clarsimp)
+    done
+next
+  case (v_sem_case_m \<xi> \<gamma> x t v m m' n)
+  then show ?case 
+    apply -
+    apply (erule v_sem_caseE)
+     apply (rename_tac a)
+     apply (drule_tac x = "VSum t a" in meta_spec; clarsimp)
+    apply (rename_tac a b)
+    apply (drule_tac x = "VSum a b" in meta_spec)
+    apply (elim meta_impE; assumption?)
+    apply (rule FalseE)
+    by simp
+next
+  case (v_sem_case_nm \<xi> \<gamma> x t' v t n n' m)
+  then show ?case
+    apply -
+    apply (erule v_sem_caseE)
+     apply (rename_tac a)
+     apply (drule_tac x = "VSum t a" in meta_spec)
+     apply (elim meta_impE; assumption?)
+     apply (rule FalseE)
+     apply simp
+    by clarsimp
+next
+  case (v_sem_if \<xi> \<gamma> x b t e r)
+  then show ?case 
+    apply -
+    apply (erule v_sem_ifE)
+    apply (rename_tac b')
+    by (drule_tac x = "VPrim (LBool b')" in meta_spec; clarsimp)
+next
+  case (v_sem_take \<xi> \<gamma> x fs f e e')
+  then show ?case 
+    apply -
+    apply (erule v_sem_takeE)
+    apply (rename_tac fs')
+    by (drule_tac x = "VRecord fs'" in meta_spec; clarsimp)
+next
+  case (v_sem_put \<xi> \<gamma> x fs e e' f)
+  then show ?case 
+    apply -
+    apply (erule v_sem_putE)
+    apply (rename_tac fs' v)
+    by (drule_tac x = "VRecord fs'" in meta_spec; clarsimp)
+next
+  case (v_sem_split \<xi> \<gamma> x a b e e')
+  then show ?case 
+    apply -
+    apply (erule v_sem_splitE)
+    apply (rename_tac a' b')
+    by (drule_tac x = "VProduct a' b'" in meta_spec; clarsimp)
+next
+  case (v_sem_prim \<xi> \<gamma> as as' p)
+  then show ?case by (fastforce elim!: v_sem_primE)
+next
+  case (v_sem_struct \<xi> \<gamma> xs vs ts)
+  then show ?case by (metis v_sem_structE)
+next
+  case (v_sem_promote \<xi> \<gamma> e e' t')
+  then show ?case by (metis v_sem_promoteE)
+next
+  case (v_sem_all_empty \<xi> \<gamma>)
+  then show ?case by (metis v_sem_all_NilE)
+next
+case (v_sem_all_cons \<xi> \<gamma> x v xs vs)
+  then show ?case by (metis v_sem_all_ConsE)
+qed (fastforce elim!: v_sem_elims)+
+
+lemma v_sem_v_sem_all_determ_not:
+  "\<lbrakk>\<xi>a, \<gamma> \<turnstile> e  \<Down> v; v \<noteq> v'; \<xi>v_determ \<xi>a\<rbrakk> \<Longrightarrow> \<not> (\<xi>a, \<gamma> \<turnstile> e \<Down> v')" and
+  "\<lbrakk>\<xi>a , \<gamma> \<turnstile>* es \<Down> vs; vs \<noteq> vs'; \<xi>v_determ \<xi>a\<rbrakk> \<Longrightarrow> \<not> (\<xi>a, \<gamma> \<turnstile>* es \<Down> vs')"
+   apply clarsimp
+   apply (erule notE)
+   apply (rule v_sem_v_sem_all_determ(1); assumption)
+  apply clarsimp
+  apply (erule notE)
+  apply (rule v_sem_v_sem_all_determ(2); assumption)
+  done
+
+
+context value_sem begin
+
+
+lemma \<xi>vle_matches:
+  "\<lbrakk>\<xi>b matches \<Xi>'; \<xi>vle \<xi>a \<xi>b\<rbrakk> \<Longrightarrow> \<xi>a matches \<Xi>'"
+  unfolding proc_env_matches_def \<xi>vle_def
+  apply clarsimp
+  apply (erule_tac x = f in allE; clarsimp)
+  apply (erule_tac x = \<tau>s in allE; clarsimp)
+  apply (erule_tac x = v in allE; clarsimp)
+  apply (erule_tac x = v' in allE; clarsimp)
+  apply (drule_tac c = "(f, v, v')" in  subsetD; simp)
+  done
+
+end (* of context *)
+end
